example/Escrow2.thy
@@ -13,7 +13,7 @@ contract Escrow {
     uint256 amount;
 
     function Escrow(address _buyer, address _seller, uint256 _amount) public {
-            require (amount > 0);
+            require (amount > 0 && _buyer != 0 && _seller != 0);
             buyer = _buyer;
             seller = _seller;
             arbiter = msg.sender;
@@ -26,12 +26,12 @@ contract Escrow {
     }
 
     function refund() public {
-        require (msg.sender == arbiter);
+        require (amount == 0 && msg.sender == arbiter);
         selfdestruct(buyer);
     }
 
     function pay() public {
-        require (msg.sender == arbiter);
+        require (amount == 0 && msg.sender == arbiter);
         selfdestruct(seller);
     }
 }
@@ -45,150 +45,167 @@ Compiled with:
 
 
 *)
-value"(parse_bytecode ''6060604052600436106100565763ffffffff7c01000000000000000000000000000000000000000000000000000000006000350416631b9265b8811461005b578063590e1ae3146100705780638f9595d414610083575b600080fd5b341561006657600080fd5b61006e61008b565b005b341561007b57600080fd5b61006e6100ce565b61006e610111565b6002543373ffffffffffffffffffffffffffffffffffffffff9081169116146100b357600080fd5b60015473ffffffffffffffffffffffffffffffffffffffff16ff5b6002543373ffffffffffffffffffffffffffffffffffffffff9081169116146100f657600080fd5b60005473ffffffffffffffffffffffffffffffffffffffff16ff5b6000600354118015610124575060035434145b801561014b57506000543373ffffffffffffffffffffffffffffffffffffffff9081169116145b151561015657600080fd5b60006003555600a165627a7a72305820629d81bfc4f4b93d45c4a23ece82e54d086d3412bb0f9a65747d991d091292610029'')"
+value"(parse_bytecode ''606060405263ffffffff7c01000000000000000000000000000000000000000000000000000000006000350416631b9265b88114610052578063590e1ae3146100675780638f9595d41461007a57600080fd5b341561005d57600080fd5b610065610082565b005b341561007257600080fd5b6100656100d3565b610065610124565b6003541580156100ad57506002543373ffffffffffffffffffffffffffffffffffffffff9081169116145b15156100b857600080fd5b60015473ffffffffffffffffffffffffffffffffffffffff16ff5b6003541580156100fe57506002543373ffffffffffffffffffffffffffffffffffffffff9081169116145b151561010957600080fd5b60005473ffffffffffffffffffffffffffffffffffffffff16ff5b6000600354118015610137575060035434145b801561015e57506000543373ffffffffffffffffffffffffffffffffffffffff9081169116145b151561016957600080fd5b60006003555600a165627a7a7230582029f2f38b5b84c1c55e91aaca3d9362e635c88ad7e3be217a7183f3cccee1aed40029'')"
 
 definition insts_ex where
-"insts_ex == [Stack (PUSH_N [0x60]), Stack (PUSH_N [0x40]), Memory MSTORE, Stack (PUSH_N [4]), Info CALLDATASIZE,
-  Arith inst_LT, Stack (PUSH_N [0, 0x56]), Pc JUMPI, Stack (PUSH_N [0xFF, 0xFF, 0xFF, 0xFF]),
+"insts_ex == [Stack (PUSH_N [0x60]), Stack (PUSH_N [0x40]), Memory MSTORE, Stack (PUSH_N [0xFF, 0xFF, 0xFF, 0xFF]),
   Stack (PUSH_N [1, 0, 0, 0, 0, 0, 0, 0, 0, 0, 0, 0, 0, 0, 0, 0, 0, 0, 0, 0, 0, 0, 0, 0, 0, 0, 0, 0, 0]),
-  Stack (PUSH_N [0]), Stack CALLDATALOAD, Arith DIV, Bits inst_AND, Stack (PUSH_N [0x1B, 0x92, 0x65, 0xB8]),
-  Dup 1, Arith inst_EQ, Stack (PUSH_N [0, 0x5B]), Pc JUMPI, Dup 0, Stack (PUSH_N [0x59, 0xE, 0x1A, 0xE3]),
-  Arith inst_EQ, Stack (PUSH_N [0, 0x70]), Pc JUMPI, Dup 0, Stack (PUSH_N [0x8F, 0x95, 0x95, 0xD4]),
-  Arith inst_EQ, Stack (PUSH_N [0, 0x83]), Pc JUMPI, Pc JUMPDEST, Stack (PUSH_N [0]), Dup 0, Unknown 0xFD,
-  Pc JUMPDEST, Info CALLVALUE, Arith ISZERO, Stack (PUSH_N [0, 0x66]), Pc JUMPI, Stack (PUSH_N [0]), Dup 0,
-  Unknown 0xFD, Pc JUMPDEST, Stack (PUSH_N [0, 0x6E]), Stack (PUSH_N [0, 0x8B]), Pc JUMP, Pc JUMPDEST,
-  Misc STOP, Pc JUMPDEST, Info CALLVALUE, Arith ISZERO, Stack (PUSH_N [0, 0x7B]), Pc JUMPI, Stack (PUSH_N [0]),
-  Dup 0, Unknown 0xFD, Pc JUMPDEST, Stack (PUSH_N [0, 0x6E]), Stack (PUSH_N [0, 0xCE]), Pc JUMP, Pc JUMPDEST,
-  Stack (PUSH_N [0, 0x6E]), Stack (PUSH_N [1, 0x11]), Pc JUMP, Pc JUMPDEST, Stack (PUSH_N [2]), Storage SLOAD,
+  Stack (PUSH_N [0]), Stack CALLDATALOAD, Arith DIV, Bits inst_AND,
+  Stack (PUSH_N [0x1B, 0x92, 0x65, 0xB8]), Dup 1, Arith inst_EQ, Stack (PUSH_N [0, 0x52]), Pc JUMPI, Dup 0,
+  Stack (PUSH_N [0x59, 0xE, 0x1A, 0xE3]), Arith inst_EQ, Stack (PUSH_N [0, 0x67]), Pc JUMPI, Dup 0,
+  Stack (PUSH_N [0x8F, 0x95, 0x95, 0xD4]), Arith inst_EQ, Stack (PUSH_N [0, 0x7A]), Pc JUMPI,
+  Stack (PUSH_N [0]), Dup 0, Unknown 0xFD, Pc JUMPDEST, Info CALLVALUE, Arith ISZERO,
+  Stack (PUSH_N [0, 0x5D]), Pc JUMPI, Stack (PUSH_N [0]), Dup 0, Unknown 0xFD, Pc JUMPDEST,
+  Stack (PUSH_N [0, 0x65]), Stack (PUSH_N [0, 0x82]), Pc JUMP, Pc JUMPDEST, Misc STOP, Pc JUMPDEST,
+  Info CALLVALUE, Arith ISZERO, Stack (PUSH_N [0, 0x72]), Pc JUMPI, Stack (PUSH_N [0]), Dup 0,
+  Unknown 0xFD, Pc JUMPDEST, Stack (PUSH_N [0, 0x65]), Stack (PUSH_N [0, 0xD3]), Pc JUMP, Pc JUMPDEST,
+  Stack (PUSH_N [0, 0x65]), Stack (PUSH_N [1, 0x24]), Pc JUMP, Pc JUMPDEST, Stack (PUSH_N [3]),
+  Storage SLOAD, Arith ISZERO, Dup 0, Arith ISZERO, Stack (PUSH_N [0, 0xAD]), Pc JUMPI, Stack POP,
+  Stack (PUSH_N [2]), Storage SLOAD, Info CALLER,
+  Stack (PUSH_N
+          [0xFF, 0xFF, 0xFF, 0xFF, 0xFF, 0xFF, 0xFF, 0xFF, 0xFF, 0xFF, 0xFF, 0xFF, 0xFF, 0xFF, 0xFF, 0xFF,
+           0xFF, 0xFF, 0xFF, 0xFF]),
+  Swap 0, Dup 1, Bits inst_AND, Swap 1, Bits inst_AND, Arith inst_EQ, Pc JUMPDEST, Arith ISZERO,
+  Arith ISZERO, Stack (PUSH_N [0, 0xB8]), Pc JUMPI, Stack (PUSH_N [0]), Dup 0, Unknown 0xFD, Pc JUMPDEST,
+  Stack (PUSH_N [1]), Storage SLOAD,
+  Stack (PUSH_N
+          [0xFF, 0xFF, 0xFF, 0xFF, 0xFF, 0xFF, 0xFF, 0xFF, 0xFF, 0xFF, 0xFF, 0xFF, 0xFF, 0xFF, 0xFF, 0xFF,
+           0xFF, 0xFF, 0xFF, 0xFF]),
+  Bits inst_AND, Misc SUICIDE, Pc JUMPDEST, Stack (PUSH_N [3]), Storage SLOAD, Arith ISZERO, Dup 0,
+  Arith ISZERO, Stack (PUSH_N [0, 0xFE]), Pc JUMPI, Stack POP, Stack (PUSH_N [2]), Storage SLOAD,
   Info CALLER,
   Stack (PUSH_N
-          [0xFF, 0xFF, 0xFF, 0xFF, 0xFF, 0xFF, 0xFF, 0xFF, 0xFF, 0xFF, 0xFF, 0xFF, 0xFF, 0xFF, 0xFF, 0xFF, 0xFF,
-           0xFF, 0xFF, 0xFF]),
-  Swap 0, Dup 1, Bits inst_AND, Swap 1, Bits inst_AND, Arith inst_EQ, Stack (PUSH_N [0, 0xB3]), Pc JUMPI,
-  Stack (PUSH_N [0]), Dup 0, Unknown 0xFD, Pc JUMPDEST, Stack (PUSH_N [1]), Storage SLOAD,
+          [0xFF, 0xFF, 0xFF, 0xFF, 0xFF, 0xFF, 0xFF, 0xFF, 0xFF, 0xFF, 0xFF, 0xFF, 0xFF, 0xFF, 0xFF, 0xFF,
+           0xFF, 0xFF, 0xFF, 0xFF]),
+  Swap 0, Dup 1, Bits inst_AND, Swap 1, Bits inst_AND, Arith inst_EQ, Pc JUMPDEST, Arith ISZERO,
+  Arith ISZERO, Stack (PUSH_N [1, 9]), Pc JUMPI, Stack (PUSH_N [0]), Dup 0, Unknown 0xFD, Pc JUMPDEST,
+  Stack (PUSH_N [0]), Storage SLOAD,
   Stack (PUSH_N
-          [0xFF, 0xFF, 0xFF, 0xFF, 0xFF, 0xFF, 0xFF, 0xFF, 0xFF, 0xFF, 0xFF, 0xFF, 0xFF, 0xFF, 0xFF, 0xFF, 0xFF,
-           0xFF, 0xFF, 0xFF]),
-  Bits inst_AND, Misc SUICIDE, Pc JUMPDEST, Stack (PUSH_N [2]), Storage SLOAD, Info CALLER,
-  Stack (PUSH_N
-          [0xFF, 0xFF, 0xFF, 0xFF, 0xFF, 0xFF, 0xFF, 0xFF, 0xFF, 0xFF, 0xFF, 0xFF, 0xFF, 0xFF, 0xFF, 0xFF, 0xFF,
-           0xFF, 0xFF, 0xFF]),
-  Swap 0, Dup 1, Bits inst_AND, Swap 1, Bits inst_AND, Arith inst_EQ, Stack (PUSH_N [0, 0xF6]), Pc JUMPI,
-  Stack (PUSH_N [0]), Dup 0, Unknown 0xFD, Pc JUMPDEST, Stack (PUSH_N [0]), Storage SLOAD,
-  Stack (PUSH_N
-          [0xFF, 0xFF, 0xFF, 0xFF, 0xFF, 0xFF, 0xFF, 0xFF, 0xFF, 0xFF, 0xFF, 0xFF, 0xFF, 0xFF, 0xFF, 0xFF, 0xFF,
-           0xFF, 0xFF, 0xFF]),
+          [0xFF, 0xFF, 0xFF, 0xFF, 0xFF, 0xFF, 0xFF, 0xFF, 0xFF, 0xFF, 0xFF, 0xFF, 0xFF, 0xFF, 0xFF, 0xFF,
+           0xFF, 0xFF, 0xFF, 0xFF]),
   Bits inst_AND, Misc SUICIDE, Pc JUMPDEST, Stack (PUSH_N [0]), Stack (PUSH_N [3]), Storage SLOAD,
-  Arith inst_GT, Dup 0, Arith ISZERO, Stack (PUSH_N [1, 0x24]), Pc JUMPI, Stack POP, Stack (PUSH_N [3]),
-  Storage SLOAD, Info CALLVALUE, Arith inst_EQ, Pc JUMPDEST, Dup 0, Arith ISZERO, Stack (PUSH_N [1, 0x4B]),
+  Arith inst_GT, Dup 0, Arith ISZERO, Stack (PUSH_N [1, 0x37]), Pc JUMPI, Stack POP, Stack (PUSH_N [3]),
+  Storage SLOAD, Info CALLVALUE, Arith inst_EQ, Pc JUMPDEST, Dup 0, Arith ISZERO, Stack (PUSH_N [1, 0x5E]),
   Pc JUMPI, Stack POP, Stack (PUSH_N [0]), Storage SLOAD, Info CALLER,
   Stack (PUSH_N
-          [0xFF, 0xFF, 0xFF, 0xFF, 0xFF, 0xFF, 0xFF, 0xFF, 0xFF, 0xFF, 0xFF, 0xFF, 0xFF, 0xFF, 0xFF, 0xFF, 0xFF,
-           0xFF, 0xFF, 0xFF]),
-  Swap 0, Dup 1, Bits inst_AND, Swap 1, Bits inst_AND, Arith inst_EQ, Pc JUMPDEST, Arith ISZERO, Arith ISZERO,
-  Stack (PUSH_N [1, 0x56]), Pc JUMPI, Stack (PUSH_N [0]), Dup 0, Unknown 0xFD, Pc JUMPDEST, Stack (PUSH_N [0]),
-  Stack (PUSH_N [3]), Storage SSTORE, Pc JUMP, Misc STOP, Log LOG1,
-  Stack (PUSH_N [0x62, 0x7A, 0x7A, 0x72, 0x30, 0x58]), Arith SHA3, Stack (PUSH_N [0x9D, 0x81, 0xBF]),
-  Unknown 0xC4, Misc DELEGATECALL, Unknown 0xB9, Unknown 0x3D, Info GASLIMIT, Unknown 0xC4, Log LOG2,
-  Unknown 0x3E, Unknown 0xCE, Dup 2, Unknown 0xE5, Unknown 0x4D, Arith ADDMOD,
-  Stack (PUSH_N [0x34, 0x12, 0xBB, 0xF, 0x9A, 0x65, 0x74, 0x7D, 0x99, 0x1D, 9, 0x12, 0x92, 0x61]), Misc STOP,
-  Unknown 0x29]"
+          [0xFF, 0xFF, 0xFF, 0xFF, 0xFF, 0xFF, 0xFF, 0xFF, 0xFF, 0xFF, 0xFF, 0xFF, 0xFF, 0xFF, 0xFF, 0xFF,
+           0xFF, 0xFF, 0xFF, 0xFF]),
+  Swap 0, Dup 1, Bits inst_AND, Swap 1, Bits inst_AND, Arith inst_EQ, Pc JUMPDEST, Arith ISZERO,
+  Arith ISZERO, Stack (PUSH_N [1, 0x69]), Pc JUMPI, Stack (PUSH_N [0]), Dup 0, Unknown 0xFD, Pc JUMPDEST,
+  Stack (PUSH_N [0]), Stack (PUSH_N [3]), Storage SSTORE, Pc JUMP, Misc STOP, Log LOG1,
+  Stack (PUSH_N [0x62, 0x7A, 0x7A, 0x72, 0x30, 0x58]), Arith SHA3, Unknown 0x29, Misc CALLCODE,
+  Misc RETURN, Dup 0xB, Pc JUMPDEST, Dup 4, Unknown 0xC1, Unknown 0xC5, Unknown 0x5E, Swap 1, Unknown 0xAA,
+  Unknown 0xCA, Unknown 0x3D, Swap 3, Stack (PUSH_N [0xE6, 0x35, 0xC8]), Dup 0xA, Unknown 0xD7,
+  Unknown 0xE3, Unknown 0xBE, Unknown 0x21,
+  Stack (PUSH_N [0x71, 0x83, 0xF3, 0xCC, 0xCE, 0xE1, 0xAE, 0xD4, 0, 0x29])]"
 value "length insts_ex"
-(* 171 instructions *)
+(* 191 instructions *)
 
 lemma
- "parse_bytecode ''6060604052600436106100565763ffffffff7c01000000000000000000000000000000000000000000000000000000006000350416631b9265b8811461005b578063590e1ae3146100705780638f9595d414610083575b600080fd5b341561006657600080fd5b61006e61008b565b005b341561007b57600080fd5b61006e6100ce565b61006e610111565b6002543373ffffffffffffffffffffffffffffffffffffffff9081169116146100b357600080fd5b60015473ffffffffffffffffffffffffffffffffffffffff16ff5b6002543373ffffffffffffffffffffffffffffffffffffffff9081169116146100f657600080fd5b60005473ffffffffffffffffffffffffffffffffffffffff16ff5b6000600354118015610124575060035434145b801561014b57506000543373ffffffffffffffffffffffffffffffffffffffff9081169116145b151561015657600080fd5b60006003555600a165627a7a72305820629d81bfc4f4b93d45c4a23ece82e54d086d3412bb0f9a65747d991d091292610029'' = insts_ex"
+ "parse_bytecode ''606060405263ffffffff7c01000000000000000000000000000000000000000000000000000000006000350416631b9265b88114610052578063590e1ae3146100675780638f9595d41461007a57600080fd5b341561005d57600080fd5b610065610082565b005b341561007257600080fd5b6100656100d3565b610065610124565b6003541580156100ad57506002543373ffffffffffffffffffffffffffffffffffffffff9081169116145b15156100b857600080fd5b60015473ffffffffffffffffffffffffffffffffffffffff16ff5b6003541580156100fe57506002543373ffffffffffffffffffffffffffffffffffffffff9081169116145b151561010957600080fd5b60005473ffffffffffffffffffffffffffffffffffffffff16ff5b6000600354118015610137575060035434145b801561015e57506000543373ffffffffffffffffffffffffffffffffffffffff9081169116145b151561016957600080fd5b60006003555600a165627a7a7230582029f2f38b5b84c1c55e91aaca3d9362e635c88ad7e3be217a7183f3cccee1aed40029'' = insts_ex"
   unfolding insts_ex_def
   by eval
 
 definition "blocks_escrow == build_blocks insts_ex"
 value "blocks_escrow"
 lemma blocks_escrow_simp:
- "blocks_escrow = [(0, [(0, Stack (PUSH_N [0x60])), (2, Stack (PUSH_N [0x40])), (4, Memory MSTORE), (5, Stack (PUSH_N [4])),
-       (7, Info CALLDATASIZE), (8, Arith inst_LT), (9, Stack (PUSH_N [0, 0x56]))],
+ "blocks_escrow = [(0, [(0, Stack (PUSH_N [0x60])), (2, Stack (PUSH_N [0x40])), (4, Memory MSTORE),
+       (5, Stack (PUSH_N [0xFF, 0xFF, 0xFF, 0xFF])),
+       (10, Stack (PUSH_N
+                    [1, 0, 0, 0, 0, 0, 0, 0, 0, 0, 0, 0, 0, 0, 0, 0, 0, 0, 0, 0, 0, 0, 0, 0, 0, 0, 0, 0,
+                     0])),
+       (40, Stack (PUSH_N [0])), (42, Stack CALLDATALOAD), (43, Arith DIV), (44, Bits inst_AND),
+       (45, Stack (PUSH_N [0x1B, 0x92, 0x65, 0xB8])), (50, Dup 1), (51, Arith inst_EQ),
+       (52, Stack (PUSH_N [0, 0x52]))],
    Jumpi),
-  (13, [(13, Stack (PUSH_N [0xFF, 0xFF, 0xFF, 0xFF])),
-        (18, Stack (PUSH_N
-                     [1, 0, 0, 0, 0, 0, 0, 0, 0, 0, 0, 0, 0, 0, 0, 0, 0, 0, 0, 0, 0, 0, 0, 0, 0, 0, 0, 0, 0])),
-        (48, Stack (PUSH_N [0])), (50, Stack CALLDATALOAD), (51, Arith DIV), (52, Bits inst_AND),
-        (53, Stack (PUSH_N [0x1B, 0x92, 0x65, 0xB8])), (58, Dup 1), (59, Arith inst_EQ),
-        (60, Stack (PUSH_N [0, 0x5B]))],
+  (56, [(56, Dup 0), (57, Stack (PUSH_N [0x59, 0xE, 0x1A, 0xE3])), (62, Arith inst_EQ),
+        (63, Stack (PUSH_N [0, 0x67]))],
    Jumpi),
-  (64, [(64, Dup 0), (65, Stack (PUSH_N [0x59, 0xE, 0x1A, 0xE3])), (70, Arith inst_EQ),
-        (71, Stack (PUSH_N [0, 0x70]))],
+  (67, [(67, Dup 0), (68, Stack (PUSH_N [0x8F, 0x95, 0x95, 0xD4])), (73, Arith inst_EQ),
+        (74, Stack (PUSH_N [0, 0x7A]))],
    Jumpi),
-  (75, [(75, Dup 0), (76, Stack (PUSH_N [0x8F, 0x95, 0x95, 0xD4])), (81, Arith inst_EQ),
-        (82, Stack (PUSH_N [0, 0x83]))],
+  (78, [(78, Stack (PUSH_N [0])), (80, Dup 0), (81, Unknown 0xFD)], Terminal),
+  (82, [(82, Pc JUMPDEST), (83, Info CALLVALUE), (84, Arith ISZERO), (85, Stack (PUSH_N [0, 0x5D]))],
    Jumpi),
-  (86, [(86, Pc JUMPDEST), (87, Stack (PUSH_N [0])), (89, Dup 0), (90, Unknown 0xFD)], Terminal),
-  (91, [(91, Pc JUMPDEST), (92, Info CALLVALUE), (93, Arith ISZERO), (94, Stack (PUSH_N [0, 0x66]))], Jumpi),
-  (98, [(98, Stack (PUSH_N [0])), (100, Dup 0), (101, Unknown 0xFD)], Terminal),
-  (102, [(102, Pc JUMPDEST), (103, Stack (PUSH_N [0, 0x6E])), (106, Stack (PUSH_N [0, 0x8B]))], Jump),
-  (110, [(110, Pc JUMPDEST), (111, Misc STOP)], Terminal),
-  (112, [(112, Pc JUMPDEST), (113, Info CALLVALUE), (114, Arith ISZERO), (115, Stack (PUSH_N [0, 0x7B]))],
+  (89, [(89, Stack (PUSH_N [0])), (91, Dup 0), (92, Unknown 0xFD)], Terminal),
+  (93, [(93, Pc JUMPDEST), (94, Stack (PUSH_N [0, 0x65])), (97, Stack (PUSH_N [0, 0x82]))], Jump),
+  (101, [(101, Pc JUMPDEST), (102, Misc STOP)], Terminal),
+  (103, [(103, Pc JUMPDEST), (104, Info CALLVALUE), (105, Arith ISZERO), (106, Stack (PUSH_N [0, 0x72]))],
    Jumpi),
-  (119, [(119, Stack (PUSH_N [0])), (121, Dup 0), (122, Unknown 0xFD)], Terminal),
-  (123, [(123, Pc JUMPDEST), (124, Stack (PUSH_N [0, 0x6E])), (127, Stack (PUSH_N [0, 0xCE]))], Jump),
-  (131, [(131, Pc JUMPDEST), (132, Stack (PUSH_N [0, 0x6E])), (135, Stack (PUSH_N [1, 0x11]))], Jump),
-  (139, [(139, Pc JUMPDEST), (140, Stack (PUSH_N [2])), (142, Storage SLOAD), (143, Info CALLER),
-         (144, Stack (PUSH_N
+  (110, [(110, Stack (PUSH_N [0])), (112, Dup 0), (113, Unknown 0xFD)], Terminal),
+  (114, [(114, Pc JUMPDEST), (115, Stack (PUSH_N [0, 0x65])), (118, Stack (PUSH_N [0, 0xD3]))], Jump),
+  (122, [(122, Pc JUMPDEST), (123, Stack (PUSH_N [0, 0x65])), (126, Stack (PUSH_N [1, 0x24]))], Jump),
+  (130, [(130, Pc JUMPDEST), (131, Stack (PUSH_N [3])), (133, Storage SLOAD), (134, Arith ISZERO),
+         (135, Dup 0), (136, Arith ISZERO), (137, Stack (PUSH_N [0, 0xAD]))],
+   Jumpi),
+  (141, [(141, Stack POP), (142, Stack (PUSH_N [2])), (144, Storage SLOAD), (145, Info CALLER),
+         (146, Stack (PUSH_N
                        [0xFF, 0xFF, 0xFF, 0xFF, 0xFF, 0xFF, 0xFF, 0xFF, 0xFF, 0xFF, 0xFF, 0xFF, 0xFF, 0xFF,
                         0xFF, 0xFF, 0xFF, 0xFF, 0xFF, 0xFF])),
-         (165, Swap 0), (166, Dup 1), (167, Bits inst_AND), (168, Swap 1), (169, Bits inst_AND),
-         (170, Arith inst_EQ), (171, Stack (PUSH_N [0, 0xB3]))],
-   Jumpi),
-  (175, [(175, Stack (PUSH_N [0])), (177, Dup 0), (178, Unknown 0xFD)], Terminal),
-  (179, [(179, Pc JUMPDEST), (180, Stack (PUSH_N [1])), (182, Storage SLOAD),
-         (183, Stack (PUSH_N
-                       [0xFF, 0xFF, 0xFF, 0xFF, 0xFF, 0xFF, 0xFF, 0xFF, 0xFF, 0xFF, 0xFF, 0xFF, 0xFF, 0xFF,
-                        0xFF, 0xFF, 0xFF, 0xFF, 0xFF, 0xFF])),
-         (204, Bits inst_AND), (205, Misc SUICIDE)],
-   Terminal),
-  (206, [(206, Pc JUMPDEST), (207, Stack (PUSH_N [2])), (209, Storage SLOAD), (210, Info CALLER),
-         (211, Stack (PUSH_N
-                       [0xFF, 0xFF, 0xFF, 0xFF, 0xFF, 0xFF, 0xFF, 0xFF, 0xFF, 0xFF, 0xFF, 0xFF, 0xFF, 0xFF,
-                        0xFF, 0xFF, 0xFF, 0xFF, 0xFF, 0xFF])),
-         (232, Swap 0), (233, Dup 1), (234, Bits inst_AND), (235, Swap 1), (236, Bits inst_AND),
-         (237, Arith inst_EQ), (238, Stack (PUSH_N [0, 0xF6]))],
-   Jumpi),
-  (242, [(242, Stack (PUSH_N [0])), (244, Dup 0), (245, Unknown 0xFD)], Terminal),
-  (246, [(246, Pc JUMPDEST), (247, Stack (PUSH_N [0])), (249, Storage SLOAD),
-         (250, Stack (PUSH_N
-                       [0xFF, 0xFF, 0xFF, 0xFF, 0xFF, 0xFF, 0xFF, 0xFF, 0xFF, 0xFF, 0xFF, 0xFF, 0xFF, 0xFF,
-                        0xFF, 0xFF, 0xFF, 0xFF, 0xFF, 0xFF])),
-         (271, Bits inst_AND), (272, Misc SUICIDE)],
-   Terminal),
-  (273, [(273, Pc JUMPDEST), (274, Stack (PUSH_N [0])), (276, Stack (PUSH_N [3])), (278, Storage SLOAD),
-         (279, Arith inst_GT), (280, Dup 0), (281, Arith ISZERO), (282, Stack (PUSH_N [1, 0x24]))],
-   Jumpi),
-  (286, [(286, Stack POP), (287, Stack (PUSH_N [3])), (289, Storage SLOAD), (290, Info CALLVALUE),
-         (291, Arith inst_EQ)],
+         (167, Swap 0), (168, Dup 1), (169, Bits inst_AND), (170, Swap 1), (171, Bits inst_AND),
+         (172, Arith inst_EQ)],
    Next),
-  (292, [(292, Pc JUMPDEST), (293, Dup 0), (294, Arith ISZERO), (295, Stack (PUSH_N [1, 0x4B]))], Jumpi),
-  (299, [(299, Stack POP), (300, Stack (PUSH_N [0])), (302, Storage SLOAD), (303, Info CALLER),
-         (304, Stack (PUSH_N
+  (173, [(173, Pc JUMPDEST), (174, Arith ISZERO), (175, Arith ISZERO), (176, Stack (PUSH_N [0, 0xB8]))],
+   Jumpi),
+  (180, [(180, Stack (PUSH_N [0])), (182, Dup 0), (183, Unknown 0xFD)], Terminal),
+  (184, [(184, Pc JUMPDEST), (185, Stack (PUSH_N [1])), (187, Storage SLOAD),
+         (188, Stack (PUSH_N
                        [0xFF, 0xFF, 0xFF, 0xFF, 0xFF, 0xFF, 0xFF, 0xFF, 0xFF, 0xFF, 0xFF, 0xFF, 0xFF, 0xFF,
                         0xFF, 0xFF, 0xFF, 0xFF, 0xFF, 0xFF])),
-         (325, Swap 0), (326, Dup 1), (327, Bits inst_AND), (328, Swap 1), (329, Bits inst_AND),
-         (330, Arith inst_EQ)],
+         (209, Bits inst_AND), (210, Misc SUICIDE)],
+   Terminal),
+  (211, [(211, Pc JUMPDEST), (212, Stack (PUSH_N [3])), (214, Storage SLOAD), (215, Arith ISZERO),
+         (216, Dup 0), (217, Arith ISZERO), (218, Stack (PUSH_N [0, 0xFE]))],
+   Jumpi),
+  (222, [(222, Stack POP), (223, Stack (PUSH_N [2])), (225, Storage SLOAD), (226, Info CALLER),
+         (227, Stack (PUSH_N
+                       [0xFF, 0xFF, 0xFF, 0xFF, 0xFF, 0xFF, 0xFF, 0xFF, 0xFF, 0xFF, 0xFF, 0xFF, 0xFF, 0xFF,
+                        0xFF, 0xFF, 0xFF, 0xFF, 0xFF, 0xFF])),
+         (248, Swap 0), (249, Dup 1), (250, Bits inst_AND), (251, Swap 1), (252, Bits inst_AND),
+         (253, Arith inst_EQ)],
    Next),
-  (331, [(331, Pc JUMPDEST), (332, Arith ISZERO), (333, Arith ISZERO), (334, Stack (PUSH_N [1, 0x56]))], Jumpi),
-  (338, [(338, Stack (PUSH_N [0])), (340, Dup 0), (341, Unknown 0xFD)], Terminal),
-  (342, [(342, Pc JUMPDEST), (343, Stack (PUSH_N [0])), (345, Stack (PUSH_N [3])), (347, Storage SSTORE)],
+  (254, [(254, Pc JUMPDEST), (255, Arith ISZERO), (256, Arith ISZERO), (257, Stack (PUSH_N [1, 9]))],
+   Jumpi),
+  (261, [(261, Stack (PUSH_N [0])), (263, Dup 0), (264, Unknown 0xFD)], Terminal),
+  (265, [(265, Pc JUMPDEST), (266, Stack (PUSH_N [0])), (268, Storage SLOAD),
+         (269, Stack (PUSH_N
+                       [0xFF, 0xFF, 0xFF, 0xFF, 0xFF, 0xFF, 0xFF, 0xFF, 0xFF, 0xFF, 0xFF, 0xFF, 0xFF, 0xFF,
+                        0xFF, 0xFF, 0xFF, 0xFF, 0xFF, 0xFF])),
+         (290, Bits inst_AND), (291, Misc SUICIDE)],
+   Terminal),
+  (292, [(292, Pc JUMPDEST), (293, Stack (PUSH_N [0])), (295, Stack (PUSH_N [3])), (297, Storage SLOAD),
+         (298, Arith inst_GT), (299, Dup 0), (300, Arith ISZERO), (301, Stack (PUSH_N [1, 0x37]))],
+   Jumpi),
+  (305, [(305, Stack POP), (306, Stack (PUSH_N [3])), (308, Storage SLOAD), (309, Info CALLVALUE),
+         (310, Arith inst_EQ)],
+   Next),
+  (311, [(311, Pc JUMPDEST), (312, Dup 0), (313, Arith ISZERO), (314, Stack (PUSH_N [1, 0x5E]))], Jumpi),
+  (318, [(318, Stack POP), (319, Stack (PUSH_N [0])), (321, Storage SLOAD), (322, Info CALLER),
+         (323, Stack (PUSH_N
+                       [0xFF, 0xFF, 0xFF, 0xFF, 0xFF, 0xFF, 0xFF, 0xFF, 0xFF, 0xFF, 0xFF, 0xFF, 0xFF, 0xFF,
+                        0xFF, 0xFF, 0xFF, 0xFF, 0xFF, 0xFF])),
+         (344, Swap 0), (345, Dup 1), (346, Bits inst_AND), (347, Swap 1), (348, Bits inst_AND),
+         (349, Arith inst_EQ)],
+   Next),
+  (350, [(350, Pc JUMPDEST), (351, Arith ISZERO), (352, Arith ISZERO), (353, Stack (PUSH_N [1, 0x69]))],
+   Jumpi),
+  (357, [(357, Stack (PUSH_N [0])), (359, Dup 0), (360, Unknown 0xFD)], Terminal),
+  (361, [(361, Pc JUMPDEST), (362, Stack (PUSH_N [0])), (364, Stack (PUSH_N [3])), (366, Storage SSTORE)],
    Jump),
-  (349, [(349, Misc STOP)], Terminal),
-  (350, [(350, Log LOG1), (351, Stack (PUSH_N [0x62, 0x7A, 0x7A, 0x72, 0x30, 0x58])), (358, Arith SHA3),
-         (359, Stack (PUSH_N [0x9D, 0x81, 0xBF])), (363, Unknown 0xC4)],
+  (368, [(368, Misc STOP)], Terminal),
+  (369, [(369, Log LOG1), (370, Stack (PUSH_N [0x62, 0x7A, 0x7A, 0x72, 0x30, 0x58])), (377, Arith SHA3),
+         (378, Unknown 0x29)],
    Terminal),
-  (364, [(364, Misc DELEGATECALL)], Terminal), (365, [(365, Unknown 0xB9)], Terminal),
-  (366, [(366, Unknown 0x3D)], Terminal), (367, [(367, Info GASLIMIT), (368, Unknown 0xC4)], Terminal),
-  (369, [(369, Log LOG2), (370, Unknown 0x3E)], Terminal), (371, [(371, Unknown 0xCE)], Terminal),
-  (372, [(372, Dup 2), (373, Unknown 0xE5)], Terminal), (374, [(374, Unknown 0x4D)], Terminal),
-  (375, [(375, Arith ADDMOD),
-         (376, Stack (PUSH_N [0x34, 0x12, 0xBB, 0xF, 0x9A, 0x65, 0x74, 0x7D, 0x99, 0x1D, 9, 0x12, 0x92, 0x61])),
-         (391, Misc STOP)],
+  (379, [(379, Misc CALLCODE)], Terminal), (380, [(380, Misc RETURN)], Terminal),
+  (381, [(381, Dup 0xB)], Next), (382, [(382, Pc JUMPDEST), (383, Dup 4), (384, Unknown 0xC1)], Terminal),
+  (385, [(385, Unknown 0xC5)], Terminal), (386, [(386, Unknown 0x5E)], Terminal),
+  (387, [(387, Swap 1), (388, Unknown 0xAA)], Terminal), (389, [(389, Unknown 0xCA)], Terminal),
+  (390, [(390, Unknown 0x3D)], Terminal),
+  (391, [(391, Swap 3), (392, Stack (PUSH_N [0xE6, 0x35, 0xC8])), (396, Dup 0xA), (397, Unknown 0xD7)],
    Terminal),
-  (392, [(392, Unknown 0x29)], Terminal)]"
+  (398, [(398, Unknown 0xE3)], Terminal), (399, [(399, Unknown 0xBE)], Terminal),
+  (400, [(400, Unknown 0x21)], Terminal),
+  (401, [(401, Stack (PUSH_N [0x71, 0x83, 0xF3, 0xCC, 0xCE, 0xE1, 0xAE, 0xD4, 0, 0x29]))], Next)]"
   by eval
 
 definition addfund_hash :: "32 word"  where
@@ -204,9 +221,9 @@ definition return_action ::"address \<Rightarrow> address \<Rightarrow> address 
   "return_action sender buyer seller arbiter amount hash v = 
  (if hash = addfund_hash \<and> sender = buyer  \<and> v = amount \<and> amount > 0 then
     ContractReturn []
-  else if hash = refund_hash \<and> sender = arbiter \<and> v = 0 then
+  else if hash = refund_hash \<and> sender = arbiter \<and> v = 0 \<and> amount = 0 then
     ContractSuicide buyer
-  else if hash = pay_hash \<and> sender = arbiter \<and> v = 0 then
+  else if hash = pay_hash \<and> sender = arbiter \<and> v = 0 \<and> amount = 0 then
     ContractSuicide seller
   else
     ContractFail [ShouldNotHappen])"
@@ -322,7 +339,6 @@ shows
    apply ((block_vcg2)[1])
    apply ((block_vcg2)[1])
    apply ((block_vcg2)[1])
-   apply ((block_vcg2)[1])
   apply (split_conds)
 (* 1*)
   apply (clarsimp)+
@@ -339,12 +355,14 @@ shows
    apply ((block_vcg2)[1])
    apply ((block_vcg2)[1])
    apply ((block_vcg2)[1])
+   apply ((block_vcg2)[1])
    apply (clarsimp split: if_split_asm simp: word_rcat_simps)
   apply (clarsimp)+
   apply(split if_split, rule conjI)+
   apply(safe; clarsimp)
   apply( clarsimp)
   apply(rule exI)
+   apply ((block_vcg2)[1])
    apply ((block_vcg2)[1])
    apply ((block_vcg2)[1])
    apply ((block_vcg2)[1])
@@ -367,14 +385,25 @@ shows
   apply (clarsimp split: if_split )
   apply (rule conjI; clarsimp)
   apply (case_tac " hash = pay_hash"; clarsimp)
-  apply (case_tac "v \<noteq> 0"; clarsimp)
+  apply (case_tac "v \<noteq> 0")
    apply (rule exI)
    apply ((block_vcg2)[1])
    apply ((block_vcg2)[1])
    apply ((block_vcg2)[1])
-   apply ((block_vcg2)[1])
-   apply (clarsimp split: if_split_asm simp: word_rcat_simps)
+   apply (split_conds)
+  apply (case_tac "amount \<noteq> 0"; clarsimp)
   apply(rule exI)
+   apply ((block_vcg2)[1])
+   apply ((block_vcg2)[1])
+   apply ((block_vcg2)[1])
+   apply ((block_vcg2)[1])
+   apply ((block_vcg2)[1])
+   apply ((block_vcg2)[1])
+   apply ((block_vcg2)[1])
+   apply ((block_vcg2)[1])
+   apply (split_conds)
+  apply(rule exI)
+   apply ((block_vcg2)[1])
    apply ((block_vcg2)[1])
    apply ((block_vcg2)[1])
    apply ((block_vcg2)[1])
@@ -385,15 +414,27 @@ shows
    apply (split_conds)
 (*1*)
   apply (case_tac " hash = refund_hash"; clarsimp)
-  apply (case_tac "v \<noteq> 0"; clarsimp)
+  apply (case_tac "v \<noteq> 0")
    apply (rule exI)
    apply ((block_vcg2)[1])
    apply ((block_vcg2)[1])
    apply ((block_vcg2)[1])
    apply ((block_vcg2)[1])
-   apply ((block_vcg2)[1])
-   apply (clarsimp split: if_split_asm simp: word_rcat_simps)
+   apply (split_conds)
+  apply (case_tac "amount \<noteq> 0"; clarsimp)
   apply(rule exI)
+   apply ((block_vcg2)[1])
+   apply ((block_vcg2)[1])
+   apply ((block_vcg2)[1])
+   apply ((block_vcg2)[1])
+   apply ((block_vcg2)[1])
+   apply ((block_vcg2)[1])
+   apply ((block_vcg2)[1])
+   apply ((block_vcg2)[1])
+   apply ((block_vcg2)[1])
+   apply (split_conds)
+  apply(rule exI)
+   apply ((block_vcg2)[1])
    apply ((block_vcg2)[1])
    apply ((block_vcg2)[1])
    apply ((block_vcg2)[1])
@@ -419,23 +460,8 @@ shows
    apply ((block_vcg2)[1])
    apply ((block_vcg2)[1])
   apply ((block_vcg2)[1])
-   apply ((block_vcg2)[1])
    apply (split_conds)
   apply (rule exI)
-   apply ((block_vcg2)[1])
-   apply ((block_vcg2)[1])
-   apply ((block_vcg2)[1])
-   apply ((block_vcg2)[1])
-   apply ((block_vcg2)[1])
-   apply ((block_vcg2)[1])
-   apply ((block_vcg2)[1])
-   apply ((block_vcg2)[1])
-   apply ((block_vcg2)[1])
-   apply ((block_vcg2)[1])
-   apply ((block_vcg2)[1])
-   apply (split_conds)
-  apply (rule exI)
-   apply ((block_vcg2)[1])
    apply ((block_vcg2)[1])
    apply ((block_vcg2)[1])
    apply ((block_vcg2)[1])
@@ -458,10 +484,20 @@ shows
    apply ((block_vcg2)[1])
    apply ((block_vcg2)[1])
    apply ((block_vcg2)[1])
-   apply ((block_vcg2)[1])
    apply (split_conds)
   apply (rule exI)
    apply ((block_vcg2)[1])
+   apply ((block_vcg2)[1])
+   apply ((block_vcg2)[1])
+   apply ((block_vcg2)[1])
+   apply ((block_vcg2)[1])
+   apply ((block_vcg2)[1])
+   apply ((block_vcg2)[1])
+   apply ((block_vcg2)[1])
+   apply ((block_vcg2)[1])
+   apply ((block_vcg2)[1])
+   apply (split_conds)
+  apply (rule exI)
    apply ((block_vcg2)[1])
    apply ((block_vcg2)[1])
    apply ((block_vcg2)[1])
